Here we give the complete version of the rules in Fig. \ref{f:only-through} and 
Fig. . \ref{f:only-through} which appeared in the main paper.

\begin{figure}[t]
\footnotesize
\begin{mathpar}
\infer
	{\proves{M}{\onlyIfSingle{A}{\neg A}{A'}}}
	{
	\proves{M}{\onlyThrough{A}{\neg A}{A'}}
	}
	\quad(\textsc{Changes})
	\and
\infer
	{
	\proves{M}{A_1\ \longrightarrow\ A_1'}\\
	\proves{M}{A_2\ \longrightarrow\ A_2'}\\
	\proves{M}{A_3'\ \longrightarrow\ A_3}\\
	\proves{M}{\onlyThrough{A_1'}{A_2'}{A_3'}}
	}
	{\proves{M}{\onlyThrough{A_1}{A_2}{A_3}}}
	\quad(\textsc{$\longrightarrow$})
	\and
\infer
	{
	\proves{M}{\onlyThrough{A_1}{A_2}{A}} \\\\
	\proves{M}{\onlyThrough{A_1'}{A_2}{A'}}
	}
	{\proves{M}{\onlyThrough{A_1\ \vee\ A_1'}{A_2}{A\ \vee\ A'}}}
	\quad(\textsc{$\vee$I$_1$})
	\and
\infer
	{
	\proves{M}{\onlyThrough{A_1}{A_2}{A}} \\\\
	\proves{M}{\onlyThrough{A_1}{A_2'}{A'}}
	}
	{\proves{M}{\onlyThrough{A_1}{A_2\ \vee\ A_2'}{A\ \vee\ A'}}}
	\quad(\textsc{$\vee$I$_2$})
	\and
\infer
	{
	\proves{M}{\onlyThrough{A_1}{A'}{\prg{false}}} \\\\
	\proves{M}{\onlyThrough{A_1}{A_2}{A\ \vee\ A'}}
	}
	{\proves{M}{\onlyThrough{A_1}{A_2}{A}}}
	\quad(\textsc{$\vee$E$_1$})
	\and
\infer
	{
	\proves{M}{\onlyThrough{A'}{A_2}{\prg{false}}} \\\\
	\proves{M}{\onlyThrough{A_1}{A_2}{A\ \vee\ A'}}
	}
	{\proves{M}{\onlyThrough{A_1}{A_2}{A}}}
	\quad(\textsc{$\vee$E$_2$})
	\and
\infer
	{
	\proves{M}{\onlyThrough{A_1}{A_2}{A_3}} \\\\
	\proves{M}{\onlyThrough{A_1}{A_3}{A}}
	}
	{\proves{M}{\onlyThrough{A_1}{A_2}{A}}}
	\quad(\textsc{Trans$_1$})
	\and
\infer
	{
	\proves{M}{\onlyThrough{A_1}{A_2}{A_3}} \\\\
	\proves{M}{\onlyThrough{A_3}{A_2}{A}}
	}
	{\proves{M}{\onlyThrough{A_1}{A_2}{A}}}
	\quad(\textsc{Trans$_2$})
	\and
\infer
	{
	\proves{M}{\onlyIf{A_1}{A_2}{A}}
	}
	{\proves{M}{\onlyThrough{A_1}{A_2}{A}}}
	\quad(\textsc{If})
	\and
\infer
	{}
	{\proves{M}{\onlyThrough{A_1}{A_2}{A_2}}}
	\quad(\textsc{End})
	\and
\infer
	{
	\forall y,\; \proves{M}{\onlyThrough{([y / x]A_1)}{A_2}{A}}
	}
	{\proves{M}{\onlyThrough{\exists x. [A_1]}{A_2}{A}}}
	\quad(\textsc{$\exists_1$})
	\and
\infer
	{
	\forall y,\; \proves{M}{\onlyThrough{A_1}{([y / x]A_2)}{A}}
	}
	{\proves{M}{\onlyThrough{A_1}{A_2}{A}}}
	\quad(\textsc{$\exists_2$})
\end{mathpar}
\caption{\emph{Only Through}}
\label{app:f:only-through}
\end{figure}
\begin{figure}[t]
\footnotesize
\begin{mathpar}
\infer
	{
	\proves{M}{A_1\ \longrightarrow\ A_1'}\\
	\proves{M}{A_2\ \longrightarrow\ A_2'}\\
	\proves{M}{A_3'\ \longrightarrow\ A_3}\\
	\proves{M}{\onlyIf{A_1'}{A_2'}{A_3'}}
	}
	{\proves{M}{\onlyIf{A_1}{A_2}{A_3}}}
	\quad(\textsc{If-$\longrightarrow$})
	\and
\infer
	{
	\proves{M}{\onlyIf{A_1}{A_2}{A}} \\\\
	\proves{M}{\onlyIf{A_1'}{A_2}{A'}}
	}
	{\proves{M}{\onlyIf{A_1\ \vee\ A_1'}{A_2}{A\ \vee\ A'}}}
	\quad(\textsc{If-$\vee$I$_1$})
	\and
\infer
	{
	\proves{M}{\onlyIf{A_1}{A_2}{A}} \\\\
	\proves{M}{\onlyIf{A_1}{A_2'}{A'}}
	}
	{\proves{M}{\onlyIf{A_1}{A_2\ \vee\ A_2'}{A\ \vee\ A'}}}
	\quad(\textsc{If-$\vee$I$_2$})
	\and
\infer
	{
	\proves{M}{\onlyIf{A_1}{A_2}{A\ \vee\ A'}} \\\\
	\proves{M}{\onlyThrough{A'}{A_2}{\prg{false}}}
	}
	{\proves{M}{\onlyIf{A_1}{A_2}{A}}}
	\quad(\textsc{If-$\vee$E})
	\and
\infer
	{
	\proves{M}{\onlyIf{A_1}{A_2}{A}} \\\\
	\proves{M}{\onlyThrough{A_1}{A_2}{A'}}
	}
	{\proves{M}{\onlyIf{A_1}{A_2}{A\ \wedge\ A'}}}
	\quad(\textsc{If-$\wedge$I})
	\and
\infer
	{
	\proves{M}{\onlyThrough{A_1}{A_2}{A_3}} \\\\
	\proves{M}{\onlyIf{A_1}{A_3}{A}}
	}
	{\proves{M}{\onlyIf{A_1}{A_2}{A}}}
	\quad(\textsc{If-Trans)}
	\and
\infer
	{}
	{\proves{M}{\onlyIf{A_1}{A_2}{A_1}}}
	\quad(\textsc{If-Start})
	\and
\infer
	{
	\forall y,\; \proves{M}{\onlyIf{([y / x]A_1)}{A_2}{A}}
	}
	{\proves{M}{\onlyIf{\exists x. [A_1]}{A_2}{A}}}
	\quad(\textsc{If-$\exists_1$})
	\and
\infer
	{
	\forall y,\; \proves{M}{\onlyIf{A_1}{([y / x]A_2)}{A}}
	}
	{\proves{M}{\onlyIf{A_1}{A_2}{A}}}
	\quad(\textsc{If-$\exists_2$})
\end{mathpar}
\caption{\emph{Only If}}
\label{app:f:only-if}
\end{figure}